dist/gcc-compatible/Hacl_RSAPSS.c
@@ -24,78 +24,41 @@
 
 #include "Hacl_RSAPSS.h"
 
-inline uint64_t
-Hacl_Bignum_Multiplication_mul_carry_add_u64_st(
-  uint64_t c_in,
-  uint64_t a,
-  uint64_t b,
-  uint64_t *out
-)
+static inline void bn_from_bytes_be(uint32_t len, uint8_t *b, uint64_t *res)
 {
-  FStar_UInt128_uint128 uu____0 = FStar_UInt128_uint64_to_uint128(out[0U]);
-  FStar_UInt128_uint128
-  res =
-    FStar_UInt128_add(FStar_UInt128_add(FStar_UInt128_mul_wide(a, b),
-        FStar_UInt128_uint64_to_uint128(c_in)),
-      uu____0);
-  out[0U] = FStar_UInt128_uint128_to_uint64(res);
-  return FStar_UInt128_uint128_to_uint64(FStar_UInt128_shift_right(res, (uint32_t)64U));
-}
-
-bool Hacl_Bignum_bn_is_bit_set(uint32_t len, uint64_t *input, uint32_t ind)
-{
-  uint32_t i = ind / (uint32_t)64U;
-  uint32_t j = ind % (uint32_t)64U;
-  uint64_t tmp = input[i];
-  uint64_t tmp1 = tmp >> j & (uint64_t)1U;
-  return tmp1 == (uint64_t)1U;
-}
-
-static void bn_bit_set(uint64_t *input, uint32_t ind)
-{
-  uint32_t i = ind / (uint32_t)64U;
-  uint32_t j = ind % (uint32_t)64U;
-  input[i] = input[i] | (uint64_t)1U << j;
-}
-
-static inline bool bn_is_less(uint32_t len, uint64_t *a, uint64_t *b)
-{
-  uint64_t acc = (uint64_t)0U;
-  for (uint32_t i = (uint32_t)0U; i < len; i++)
+  uint32_t bnLen = (len - (uint32_t)1U) / (uint32_t)8U + (uint32_t)1U;
+  uint32_t tmpLen = (uint32_t)8U * bnLen;
+  KRML_CHECK_SIZE(sizeof (uint8_t), tmpLen);
+  uint8_t tmp[tmpLen];
+  memset(tmp, 0U, tmpLen * sizeof (tmp[0U]));
+  memcpy(tmp + tmpLen - len, b, len * sizeof (b[0U]));
+  for (uint32_t i = (uint32_t)0U; i < bnLen; i++)
   {
-    uint64_t beq = FStar_UInt64_eq_mask(a[i], b[i]);
-    uint64_t blt = ~FStar_UInt64_gte_mask(a[i], b[i]);
-    acc = (beq & acc) | (~beq & ((blt & (uint64_t)0xFFFFFFFFFFFFFFFFU) | (~blt & (uint64_t)0U)));
+    uint64_t *os = res;
+    uint64_t u = load64_be(tmp + (bnLen - i - (uint32_t)1U) * (uint32_t)8U);
+    uint64_t x = u;
+    os[i] = x;
   }
-  uint64_t mask = acc;
-  return mask == (uint64_t)0xFFFFFFFFFFFFFFFFU;
 }
 
-inline uint64_t Hacl_Bignum_Montgomery_mod_inv_u64(uint64_t n0)
+static inline void bn_to_bytes_be(uint32_t len, uint64_t *b, uint8_t *res)
 {
-  uint64_t alpha = (uint64_t)9223372036854775808U;
-  uint64_t beta = n0;
-  uint64_t ub = (uint64_t)0U;
-  uint64_t vb = (uint64_t)0U;
-  ub = (uint64_t)1U;
-  vb = (uint64_t)0U;
-  for (uint32_t i = (uint32_t)0U; i < (uint32_t)64U; i++)
+  uint32_t bnLen = (len - (uint32_t)1U) / (uint32_t)8U + (uint32_t)1U;
+  uint32_t tmpLen = (uint32_t)8U * bnLen;
+  KRML_CHECK_SIZE(sizeof (uint8_t), tmpLen);
+  uint8_t tmp[tmpLen];
+  memset(tmp, 0U, tmpLen * sizeof (tmp[0U]));
+  for (uint32_t i = (uint32_t)0U; i < bnLen; i++)
   {
-    uint64_t us = ub;
-    uint64_t vs = vb;
-    uint64_t u_is_odd = (uint64_t)0U - (us & (uint64_t)1U);
-    uint64_t beta_if_u_is_odd = beta & u_is_odd;
-    ub = ((us ^ beta_if_u_is_odd) >> (uint32_t)1U) + (us & beta_if_u_is_odd);
-    uint64_t alpha_if_u_is_odd = alpha & u_is_odd;
-    vb = (vs >> (uint32_t)1U) + alpha_if_u_is_odd;
+    store64_be(tmp + i * (uint32_t)8U, b[bnLen - i - (uint32_t)1U]);
   }
-  return vb;
+  memcpy(res, tmp + tmpLen - len, len * sizeof ((tmp + tmpLen - len)[0U]));
 }
 
 static void precomp_runtime(uint32_t len, uint32_t modBits, uint64_t *n, uint64_t *res)
 {
   memset(res, 0U, len * sizeof (res[0U]));
-  bn_bit_set(res, modBits - (uint32_t)1U);
+  Hacl_Bignum_bn_bit_set(len, res, modBits - (uint32_t)1U);
   for (uint32_t i0 = (uint32_t)0U; i0 < (uint32_t)128U * len + (uint32_t)129U - modBits; i0++)
   {
     KRML_CHECK_SIZE(sizeof (uint64_t), len);
@@ -330,7 +293,7 @@ bn_mod_exp(
   acc[0U] = (uint64_t)1U;
   uint32_t rLen = nLen + (uint32_t)1U;
   uint32_t bLen = (bBits - (uint32_t)1U) / (uint32_t)64U + (uint32_t)1U;
-  uint64_t nInv_u64 = Hacl_Bignum_Montgomery_mod_inv_u64(n[0U]);
+  uint64_t nInv_u64 = Hacl_Bignum_ModInv64_mod_inv_u64(n[0U]);
   KRML_CHECK_SIZE(sizeof (uint64_t), nLen);
   uint64_t r2[nLen];
   memset(r2, 0U, nLen * sizeof (r2[0U]));
@@ -531,9 +494,9 @@ rsapss_sign(
   uint64_t s[nLen];
   memset(s, 0U, nLen * sizeof (s[0U]));
   pss_encode(sLen, salt, msgLen, msg, emBits, em);
-  Hacl_Bignum_Convert_bn_from_bytes_be(emLen, em, m);
+  bn_from_bytes_be(emLen, em, m);
   bn_mod_exp(modBits, nLen, n, m, dBits, d, s);
-  Hacl_Bignum_Convert_bn_to_bytes_be(k, s, sgnt);
+  bn_to_bytes_be(k, s, sgnt);
 }
 
 static bool
@@ -562,8 +525,8 @@ rsapss_verify(
   KRML_CHECK_SIZE(sizeof (uint64_t), nLen);
   uint64_t s[nLen];
   memset(s, 0U, nLen * sizeof (s[0U]));
-  Hacl_Bignum_Convert_bn_from_bytes_be(k, sgnt, s);
-  if (bn_is_less(nLen, s, n))
+  bn_from_bytes_be(k, sgnt, s);
+  if (Hacl_Bignum_bn_is_less(nLen, s, n))
   {
     bn_mod_exp(modBits, nLen, n, s, eBits, e, m);
     bool ite;
@@ -581,7 +544,7 @@ rsapss_verify(
     if (ite)
     {
       uint64_t *m1 = m;
-      Hacl_Bignum_Convert_bn_to_bytes_be(emLen, m1, em);
+      bn_to_bytes_be(emLen, m1, em);
       return pss_verify(sLen, msgLen, msg, emBits, em);
     }
     return false;
@@ -617,69 +580,5 @@ Hacl_RSAPSS_rsapss_verify(
 )
 {
   return rsapss_verify(modBits, eBits, pkey, sLen, sgnt, msgLen, msg);
-}
-
-inline void Hacl_Bignum_Convert_bn_from_bytes_be(uint32_t len, uint8_t *b, uint64_t *res)
-{
-  uint32_t bnLen = (len - (uint32_t)1U) / (uint32_t)8U + (uint32_t)1U;
-  uint32_t tmpLen = (uint32_t)8U * bnLen;
-  KRML_CHECK_SIZE(sizeof (uint8_t), tmpLen);
-  uint8_t tmp[tmpLen];
-  memset(tmp, 0U, tmpLen * sizeof (tmp[0U]));
-  memcpy(tmp + tmpLen - len, b, len * sizeof (b[0U]));
-  for (uint32_t i = (uint32_t)0U; i < bnLen; i++)
-  {
-    uint64_t *os = res;
-    uint64_t u = load64_be(tmp + (bnLen - i - (uint32_t)1U) * (uint32_t)8U);
-    uint64_t x = u;
-    os[i] = x;
-  }
-}
-
-inline void Hacl_Bignum_Convert_bn_from_bytes_le(uint32_t len, uint8_t *b, uint64_t *res)
-{
-  uint32_t bnLen = (len - (uint32_t)1U) / (uint32_t)8U + (uint32_t)1U;
-  uint32_t tmpLen = (uint32_t)8U * bnLen;
-  KRML_CHECK_SIZE(sizeof (uint8_t), tmpLen);
-  uint8_t tmp[tmpLen];
-  memset(tmp, 0U, tmpLen * sizeof (tmp[0U]));
-  memcpy(tmp, b, len * sizeof (b[0U]));
-  for (uint32_t i = (uint32_t)0U; i < (len - (uint32_t)1U) / (uint32_t)8U + (uint32_t)1U; i++)
-  {
-    uint64_t *os = res;
-    uint8_t *bj = tmp + i * (uint32_t)8U;
-    uint64_t u = load64_le(bj);
-    uint64_t r = u;
-    uint64_t x = r;
-    os[i] = x;
-  }
-}
-
-inline void Hacl_Bignum_Convert_bn_to_bytes_be(uint32_t len, uint64_t *b, uint8_t *res)
-{
-  uint32_t bnLen = (len - (uint32_t)1U) / (uint32_t)8U + (uint32_t)1U;
-  uint32_t tmpLen = (uint32_t)8U * bnLen;
-  KRML_CHECK_SIZE(sizeof (uint8_t), tmpLen);
-  uint8_t tmp[tmpLen];
-  memset(tmp, 0U, tmpLen * sizeof (tmp[0U]));
-  for (uint32_t i = (uint32_t)0U; i < bnLen; i++)
-  {
-    store64_be(tmp + i * (uint32_t)8U, b[bnLen - i - (uint32_t)1U]);
-  }
-  memcpy(res, tmp + tmpLen - len, len * sizeof ((tmp + tmpLen - len)[0U]));
-}
-
-inline void Hacl_Bignum_Convert_bn_to_bytes_le(uint32_t len, uint64_t *b, uint8_t *res)
-{
-  uint32_t bnLen = (len - (uint32_t)1U) / (uint32_t)8U + (uint32_t)1U;
-  uint32_t tmpLen = (uint32_t)8U * bnLen;
-  KRML_CHECK_SIZE(sizeof (uint8_t), tmpLen);
-  uint8_t tmp[tmpLen];
-  memset(tmp, 0U, tmpLen * sizeof (tmp[0U]));
-  for (uint32_t i = (uint32_t)0U; i < bnLen; i++)
-  {
-    store64_le(tmp + i * (uint32_t)8U, b[i]);
-  }
-  memcpy(res, tmp, len * sizeof (tmp[0U]));
 }
 
