dist/gcc-compatible/lib/Hacl_Bignum4096_bindings.ml
@@ -20,4 +20,10 @@ module Bindings(F:Cstubs.FOREIGN) =
            ((ptr uint64_t) @->
               (uint32_t @->
                  ((ptr uint64_t) @-> ((ptr uint64_t) @-> (returning void))))))
+    let hacl_Bignum4096_new_bn_from_bytes_be =
+      foreign "Hacl_Bignum4096_new_bn_from_bytes_be"
+        (uint32_t @-> (ocaml_bytes @-> (returning (ptr uint64_t))))
+    let hacl_Bignum4096_bn_to_bytes_be =
+      foreign "Hacl_Bignum4096_bn_to_bytes_be"
+        ((ptr uint64_t) @-> (ocaml_bytes @-> (returning void)))
   end
