dist/gcc-compatible/lib/Hacl_Bignum_bindings.ml
@@ -1,0 +1,23 @@
+open Ctypes
+module Bindings(F:Cstubs.FOREIGN) =
+  struct
+    open F
+    let hacl_Bignum_Multiplication_mul_carry_add_u64_st =
+      foreign "Hacl_Bignum_Multiplication_mul_carry_add_u64_st"
+        (uint64_t @->
+           (uint64_t @->
+              (uint64_t @-> ((ptr uint64_t) @-> (returning uint64_t)))))
+    let hacl_Bignum_bn_is_bit_set =
+      foreign "Hacl_Bignum_bn_is_bit_set"
+        (uint32_t @-> ((ptr uint64_t) @-> (uint32_t @-> (returning bool))))
+    let hacl_Bignum_bn_bit_set =
+      foreign "Hacl_Bignum_bn_bit_set"
+        (uint32_t @-> ((ptr uint64_t) @-> (uint32_t @-> (returning void))))
+    let hacl_Bignum_bn_is_less =
+      foreign "Hacl_Bignum_bn_is_less"
+        (uint32_t @->
+           ((ptr uint64_t) @-> ((ptr uint64_t) @-> (returning bool))))
+    let hacl_Bignum_ModInv64_mod_inv_u64 =
+      foreign "Hacl_Bignum_ModInv64_mod_inv_u64"
+        (uint64_t @-> (returning uint64_t))
+  end
