code/rsapss/Hacl.Bignum.Convert.fst
@@ -12,8 +12,11 @@ open Hacl.Bignum.Definitions
 
 module ST = FStar.HyperStack.ST
 module LSeq = Lib.Sequence
+module B = LowStar.Buffer
 
 module S = Hacl.Spec.Bignum.Convert
+
+module HS = FStar.HyperStack
 
 
 #reset-options "--z3rlimit 50 --fuel 0 --ifuel 0"
@@ -36,7 +39,8 @@ let bn_from_bytes_be_ len b res =
   (fun j -> uint_from_bytes_be (sub b ((len -! j -! 1ul) *! 8ul) 8ul))
 
 
-val bn_from_bytes_be:
+inline_for_extraction noextract
+val mk_bn_from_bytes_be:
     len:size_t{0 < v len /\ 8 * v (blocks len 8ul) <= max_size_t}
   -> b:lbuffer uint8 len
   -> res:lbignum (blocks len 8ul) ->
@@ -45,8 +49,7 @@ val bn_from_bytes_be:
   (ensures  fun h0 _ h1 -> modifies (loc res) h0 h1 /\
     as_seq h1 res == S.bn_from_bytes_be (v len) (as_seq h0 b))
 
-[@CInline]
-let bn_from_bytes_be len b res =
+let mk_bn_from_bytes_be len b res =
   let h0 = ST.get () in
   push_frame ();
   let bnLen = blocks len 8ul in
@@ -56,6 +59,46 @@ let bn_from_bytes_be len b res =
   bn_from_bytes_be_ bnLen tmp res;
   pop_frame ()
 
+[@CInline]
+let bn_from_bytes_be = mk_bn_from_bytes_be
+
+inline_for_extraction noextract
+let new_bn_from_bytes_be_st =
+    r:HS.rid
+  -> len:size_t
+  -> b:lbuffer uint8 len ->
+  ST (B.buffer uint64)
+  (requires fun h ->
+    live h b /\
+    ST.is_eternal_region r)
+  (ensures  fun h0 res h1 ->
+    B.(modifies loc_none h0 h1) /\
+    not (B.g_is_null res) ==> (
+      0 < v len /\ 8 * v (blocks len 8ul) <= max_size_t /\
+      B.len res == blocks len 8ul /\
+      B.(fresh_loc (loc_buffer res) h0 h1) /\
+      B.(loc_includes (loc_region_only false r) (loc_buffer res)) /\
+      as_seq h1 (res <: lbignum (blocks len 8ul))  == S.bn_from_bytes_be (v len) (as_seq h0 b)))
+
+inline_for_extraction noextract
+val new_bn_from_bytes_be: new_bn_from_bytes_be_st
+
+let new_bn_from_bytes_be r len b =
+  if len = 0ul || not (blocks len 8ul <=. 0xfffffffful `FStar.UInt32.div` 8ul) then
+    B.null
+  else
+    let h0 = ST.get () in
+    let res = B.malloc r (u64 0) (blocks len 8ul) in
+    let h1 = ST.get () in
+    B.(modifies_only_not_unused_in loc_none h0 h1);
+    assert (B.len res == blocks len 8ul);
+    let res: Lib.Buffer.buffer Lib.IntTypes.uint64 = res in
+    assert (B.length res == FStar.UInt32.v (blocks len 8ul));
+    let res: lbignum (blocks len 8ul) = res in
+    mk_bn_from_bytes_be len b res;
+    let h2 = ST.get () in
+    B.(modifies_only_not_unused_in loc_none h0 h2);
+    res
 
 val bn_from_bytes_le:
     len:size_t{0 < v len /\ 8 * v (blocks len 8ul) <= max_size_t}
@@ -98,10 +141,9 @@ let bn_to_bytes_be_ len b res =
   (fun j -> uint_to_bytes_be (sub res (j *! 8ul) 8ul) b.(len -! j -! 1ul));
   assert_norm (S.bn_to_bytes_be_ (v len) (as_seq h0 b) == norm [delta] S.bn_to_bytes_be_ (v len) (as_seq h0 b))
 
-
-val bn_to_bytes_be:
-    len:size_t{0 < v len /\ 8 * v (blocks len 8ul) <= max_size_t}
-  -> b:lbignum (blocks len 8ul)
+inline_for_extraction noextract
+let bn_to_bytes_be_st (len:size_t{0 < v len /\ 8 * v (blocks len 8ul) <= max_size_t}) =
+    b:lbignum (blocks len 8ul)
   -> res:lbuffer uint8 len ->
   Stack unit
   (requires fun h ->
@@ -109,8 +151,10 @@ val bn_to_bytes_be:
   (ensures  fun h0 _ h1 -> modifies (loc res) h0 h1 /\
     as_seq h1 res == S.bn_to_bytes_be (v len) (as_seq h0 b))
 
-[@CInline]
-let bn_to_bytes_be len b res =
+inline_for_extraction noextract
+val mk_bn_to_bytes_be: len:size_t{0 < v len /\ 8 * v (blocks len 8ul) <= max_size_t} -> bn_to_bytes_be_st len
+
+let mk_bn_to_bytes_be len b res =
   let h0 = ST.get () in
   push_frame ();
   let bnLen = blocks len 8ul in
@@ -120,6 +164,9 @@ let bn_to_bytes_be len b res =
   copy res (sub tmp (tmpLen -! len) len);
   pop_frame ()
 
+/// This wrapper avoids inlining in callers to preserve the shape of the RSAPSS code.
+[@CInline]
+let bn_to_bytes_be = mk_bn_to_bytes_be
 
 val bn_to_bytes_le:
     len:size_t{0 < v len /\ 8 * v (blocks len 8ul) <= max_size_t}
