code/rsapss/Hacl.Bignum.ModInv64.fsti
@@ -1,0 +1,21 @@
+module Hacl.Bignum.ModInv64
+
+open FStar.HyperStack
+open FStar.HyperStack.ST
+open FStar.Mul
+
+open Lib.IntTypes
+open Lib.Buffer
+
+open Hacl.Bignum.Definitions
+module S = Hacl.Spec.Bignum.Montgomery
+module BN = Hacl.Bignum
+
+
+#reset-options "--z3rlimit 50 --fuel 0 --ifuel 0"
+
+val mod_inv_u64: n0:uint64 ->
+  Stack uint64
+  (requires fun h -> True)
+  (ensures  fun h0 r h1 -> modifies0 h0 h1 /\
+    r == S.mod_inv_u64 n0)
