code/rsapss/Hacl.Bignum4096.fsti
@@ -14,7 +14,12 @@ let n: BN.meta_len = 64ul
 inline_for_extraction noextract
 let lbignum = Hacl.Bignum.Definitions.lbignum
 
-[@@ Comment "Write `a + b mod 2^4096` in `res`.
+[@@ CPrologue
+"/************************/
+/* Arithmetic functions */
+/************************/\n";
+Comment
+"Write `a + b mod 2^4096` in `res`.
 
   This functions returns the carry.
 
@@ -34,4 +39,29 @@ val sub: Hacl.Bignum.Addition.bn_sub_eq_len_st n
   The outparam res is meant to be a 8192-bit bignum, i.e. uint64_t[128]."]
 val mul: a:lbignum n -> b:lbignum n -> BN.bn_mul_st a b
 
+[@@ Comment "Write `a ^ b mod n1` in `res`.
+
+  The arguments a, n1 and the outparam res are meant to be 4096-bit bignums, i.e. uint64_t[64].
+  The argument b is a bignum of any size, and bBits is an upper bound on the number of significant bits of b."]
 val mod_exp: BE.bn_mod_exp_st 4096ul n
+
+[@@ CPrologue
+"\n/********************/
+/* Loads and stores */
+/********************/\n";
+Comment
+"Load a bid-endian bignum from memory.
+
+  The argument b points to len bytes of valid memory.
+  The function returns a heap-allocated bignum of size sufficient to hold the
+    result of loading b, or NULL if the amount of required memory would exceed 4GB.
+
+  If the return value is non-null, clients must eventually call free(3) on it to
+  avoid memory leaks."]
+val new_bn_from_bytes_be: Hacl.Bignum.Convert.new_bn_from_bytes_be_st
+
+[@@ Comment "Serialize a bignum into big-endian memory.
+
+  The argument b points to a 4096-bit bignum.
+  The outparam res points to 512 bytes of valid memory."]
+val bn_to_bytes_be: Hacl.Bignum.Convert.bn_to_bytes_be_st n
